fixed move up through help

basic_types.v
@@ -2012,3 +2012,84 @@ Lemma nsucc_leq: forall G n, tr G (oof n nattp) ->
                                   ). var_solv0.
     } assumption.
 Qed.
+
+(*will have to induct on n1 here
+ and lemmas for how leq_t computes*)
+(*start here*)
+Lemma leq_trans_app n2 G n1 n3 t1 t2:
+  tr G (oof n1 nattp) ->
+  tr G (oof n2 nattp) ->
+  tr G (oof n3 nattp) ->
+  tr G (oof t1 (leq_t n1 n2)) ->
+  tr G (oof t2 (leq_t n2 n3)) ->
+  tr G (oof (leq_trans_fn_app n1 n2 n3
+                          t1 t2)
+ (leq_t n1 n3)).
+  intros. unfold leq_t. unfold leq_trans_fn_app.
+  eapply (tr_arrow_elim _ (leq_t n2 n3)); try weaken leq_type; try assumption.
+  eapply (tr_arrow_elim _ (leq_t n1 n2)); try apply tr_arrow_formation;
+    try weaken leq_type; try assumption.
+  match goal with |- tr ?G (deq ?M ?M ?T) => replace T with
+      (@subst1 obj n3
+       (arrow (leq_t (subst sh1 n1) (subst sh1 n2))
+          (arrow (leq_t (subst sh1 n2) (var 0))
+                 (app (app leqtp (subst sh1 n1)) (var 0))))) end.
+  2:{ simpsub_big. auto. } apply (tr_pi_elim _ nattp); try assumption.
+  match goal with |- tr ?G (deq ?M ?M ?T) => replace T with
+      (@subst1 obj n2
+       (pi nattp (arrow (leq_t (subst (sh 2) n1) (var 1))
+          (arrow (leq_t (var 1) (var 0))
+                 (app (app leqtp (subst (sh 2) n1)) (var 0)))))) end.
+  2:{ simpsub_big. auto. } apply (tr_pi_elim _ nattp); try assumption.
+  match goal with |- tr ?G (deq ?M ?M ?T) => replace T with
+      (@subst1 obj n1
+(pi nattp (pi nattp (arrow (leq_t (var 2) (var 1))
+          (arrow (leq_t (var 1) (var 0))
+                 (app (app leqtp (var 2)) (var 0))))))) end.
+  2:{ simpsub_big. auto. } apply (tr_pi_elim _ nattp); try assumption.
+  apply leq_trans_help. Qed.
+
+
+Definition lt_trans_fn_app n1 n2 n3 h12 h23 :=
+ (* leq_trans_app (nsucc n1) (nsucc n2) n3
+                (leq_trans_app (nsucc n1) n2 (nsucc n2) h12 (leq_nsucc n2)) (*s(n1) <= s(n2)*)
+                h23.  *) leq_trans_fn_app (nsucc n1) n2 n3 h12 h23.
+
+(*n1 < n2 (s n1 <= n2)
+ n2 <= n3
+ s n1 <= n3
+ good*)
+Lemma lt_trans_app n2 G n1 n3 t1 t2:
+  tr G (oof n1 nattp) ->
+  tr G (oof n2 nattp) ->
+  tr G (oof n3 nattp) ->
+  tr G (oof t1 (lt_t n1 n2)) ->
+  tr G (oof t2 (leq_t n2 n3)) ->
+  tr G (oof (lt_trans_fn_app n1 n2 n3
+                          t1 t2)
+            (lt_t n1 n3)).
+  intros. unfold lt_trans_fn_app. unfold lt_t.
+  unfold lttp. eapply tr_compute.
+  { apply equiv_app. apply reduce_equiv. apply reduce_app_beta;
+                                           apply reduce_id.
+    apply equiv_refl.
+  }
+  {apply equiv_refl. }
+  {apply equiv_refl. }
+  simpsub_big. apply leq_trans_app; try apply nsucc_type; try assumption. unfold lt_t in H2. unfold lttp in H2.
+  eapply (tr_compute _ _ (app
+               (app
+                  (lam
+                     (app (subst sh1 leqtp)
+                       (nsucc (var 0)))) n1)
+               n2)).
+  apply equiv_symm.
+  { apply equiv_app. apply reduce_equiv.
+    replace (app leqtp (nsucc n1)) with
+        (subst1 n1 (app leqtp (nsucc (var 0)))).
+    2:{ simpsub_big. auto. }
+    apply reduce_app_beta; try apply reduce_id.
+    apply equiv_refl.
+  }
+  {apply equiv_refl. }
+  {apply equiv_refl. } assumption. Qed.
